Iris 4.1.0 (#22)
* Bump Coq 1.18.0, stdpp 1.9.0, Iris 4.1.0 - WIP

* Bump Coq 1.18.0, stdpp 1.9.0, Iris 4.1.0

* Delete attic and interpreter

* Cleanup: move lemmas, complete some TODO

interpreter/lib/program.ml
@@ -1,2 +1,0 @@
-let parse (_filename: string): (Ast.t, string) Result.t =
-  failwith "todo"
