theories/examples/adder.v
@@ -83,7 +83,7 @@ Section adder.
     iDestruct (big_sepL2_length with "Hprog") as %Hlength.
     destruct ag as [| a0 ag]; [inversion Hlength|].
     destruct ag as [| ? ag]; [inversion Hlength|].
-    feed pose proof (contiguous_between_cons_inv_first _ _ _ _ Hcont). subst a0.
+    opose proof (contiguous_between_cons_inv_first _ _ _ _ Hcont). subst a0.
     assert (isCorrectPC_range RX g_start f_end g_start f_start).
     { intros mid [? ?]. constructor; auto. solve_addr. }
     (* move r_t2 PC *)
@@ -174,7 +174,7 @@ Section adder.
     remember af as af'.
     destruct af' as [| a0 af'];[inversion Hlength|].
     destruct af' as [| ? af'];[inversion Hlength|].
-    feed pose proof (contiguous_between_cons_inv_first _ _ _ _ Hcont). subst a0.
+    opose proof (contiguous_between_cons_inv_first _ _ _ _ Hcont). subst a0.
     assert (isCorrectPC_range RX f_start f_end f_start f_end).
     { intros ? [? ?]. constructor; auto. solve_addr. }
     (* move r_t1 PC *)
@@ -426,7 +426,7 @@ Section adder.
           iIntros (r' ? Hr'). eapply lookup_delete_Some in Hr' as [? Hr'].
           by unshelve iSpecialize ("HrV" $! r' _ _ Hr'). }
         { iPureIntro. rewrite !dom_insert_L dom_delete_L dom_insert_L.
-          rewrite regmap_full_dom //. set_solver+. } }
+          rewrite regmap_full_dom //. } }
       { cbn beta. iIntros (?) "H". iIntros (->). iDestruct "H" as "[H|%]". 2: congruence.
         iApply "H". done. } }
 
