theories/examples/interval_client_adequacy_arch.v
@@ -398,30 +398,6 @@ Section int_client_adequacy.
           {nainv: logrel_na_invs Σ}
           `{memlayout: memory_layout}.
 
-  (* Note that this tactic can only be applied on the left of the disjointness condition *)
-  Ltac union_resolve_mkregion :=
-    repeat (
-      try lazymatch goal with
-          | |- _ ∪ _ ⊆ _ =>
-            etransitivity; [ eapply union_mono_l | eapply union_mono_r ]
-          end;
-      [ first [ apply dom_mkregion_incl | reflexivity ] |..]
-    ).
-
-  (* overwrite `disjoint_map_to_list` ltac to also simplify list_to_map occurrences *)
-  (* TODO: replace original *)
-  Ltac disjoint_map_to_list :=
-    rewrite (@map_disjoint_dom _ _ (gset Addr)) ?dom_union_L;
-    eapply disjoint_mono_l;
-    rewrite ?dom_list_to_map_singleton;
-    union_resolve_mkregion;
-    try match goal with |- _ ## dom (mkregion _ _ _) =>
-      eapply disjoint_mono_r; [ apply dom_mkregion_incl | ] end;
-    try match goal with |- _ ## dom (list_to_map _ ) =>
-    rewrite dom_list_to_map_L end;
-    rewrite -?list_to_set_app_L ?dom_list_to_map_singleton;
-    apply stdpp_extra.list_to_set_disj.
-
   Lemma int_client_correct :
     Forall (λ w, is_z w = true \/ in_region w adv_start adv_end) adv_instrs →
     let filtered_map := λ (m : gmap Addr Word), filter (fun '(a, _) => a ∉ minv_dom flag_inv) m in
