theories/examples/macros.v
@@ -423,8 +423,8 @@ Section macros.
     iApply (wp_wand with "[-]").
     iApply (simple_malloc_subroutine_spec with "[- $Hmalloc $Hna $Hregs $Hr_t0 $HPC $Hr_t1]"); auto.
     { rewrite !dom_insert_L dom_delete_L Hrmap_dom.
-      rewrite !difference_difference_L !singleton_union_difference_L !all_registers_union_l.
-      f_equal. set_solver-. }
+      rewrite !difference_difference_l_L !singleton_union_difference_L !all_registers_union_l.
+      f_equal. }
     (* { lia. } *)
     iNext.
     rewrite updatePcPerm_cap_non_E.
@@ -595,8 +595,8 @@ Section macros.
     iApply (wp_wand with "[- Hφfailed Hψ]").
     iApply (simple_malloc_subroutine_spec with "[- $Hmalloc $Hna $Hregs $Hr_t0 $HPC $Hr_t1]"); auto.
     { rewrite !dom_insert_L dom_delete_L Hrmap_dom.
-      rewrite !difference_difference_L !singleton_union_difference_L !all_registers_union_l.
-      f_equal. set_solver-. }
+      rewrite !difference_difference_l_L !singleton_union_difference_L !all_registers_union_l.
+      f_equal. }
     (* { lia. } *)
     iNext.
     rewrite updatePcPerm_cap_non_E.
@@ -1150,34 +1150,6 @@ Section macros.
      given (encoded) permission. If this is not the case, the macro goes to fail,
      otherwise it continues *)
 
-  (* TODO: move this to the rules_Lea.v file. *)
-  Lemma wp_Lea_fail_none Ep pc_p pc_b pc_e pc_a w r1 rv p b e a z :
-    decodeInstrW w = Lea r1 (inr rv) →
-    isCorrectPC (WCap pc_p pc_b pc_e pc_a) →
-    (a + z)%a = None ->
-
-     {{{ ▷ PC ↦ᵣ WCap pc_p pc_b pc_e pc_a
-           ∗ ▷ pc_a ↦ₐ w
-           ∗ ▷ r1 ↦ᵣ WCap p b e a
-           ∗ ▷ rv ↦ᵣ WInt z }}}
-       Instr Executable @ Ep
-     {{{ RET FailedV; True }}}.
-  Proof.
-    iIntros (Hdecode Hvpc Hz φ) "(>HPC & >Hpc_a & >Hsrc & >Hdst) Hφ".
-    iDestruct (map_of_regs_3 with "HPC Hsrc Hdst") as "[Hmap (%&%&%)]".
-    iApply (wp_lea with "[$Hmap Hpc_a]"); eauto; simplify_map_eq; eauto.
-      by rewrite !dom_insert; set_solver+.
-    iNext. iIntros (regs' retv) "(#Hspec & Hpc_a & Hmap)".
-    iDestruct "Hspec" as %Hspec.
-    destruct Hspec as [* Hsucc | * Hsucc |].
-    { (* Success (contradiction) *) simplify_map_eq. }
-    { (* Success (contradiction) *) simplify_map_eq. }
-    { (* Failure, done *) by iApply "Hφ". }
-  Qed.
-
-  (* ------------------------------- *)
-
-
   Definition reqperm_instrs r z :=
     [
     get_wtype r_t1 r;
@@ -1586,7 +1558,7 @@ Section macros.
     iIntros (Hvpc Hcont Hact) "(>Hprog & >HPC & >Hr_t1 & >Hrcode & >Hrdata & >Hact & Hφ)".
     iDestruct (big_sepL2_length with "Hprog") as %Hlength.
     assert (act_b < act_e)%a as Hlt;[solve_addr|].
-    feed pose proof (contiguous_between_region_addrs act_b act_e) as Hcont_act. solve_addr.
+    opose proof (contiguous_between_region_addrs act_b act_e _) as Hcont_act; first solve_addr.
     unfold region_mapsto.
     remember (finz.seq_between act_b act_e) as acta.
     assert (Hact_len_a : length acta = 8).
@@ -1599,12 +1571,13 @@ Section macros.
     assert (∀ i a', acta !! i = Some a' → withinBounds act_b act_e a' = true) as Hwbact.
     { intros i a' Hsome. apply andb_true_intro. subst acta.
       apply contiguous_between_incr_addr with (i:=i) (ai:=a') in Hcont_act. 2: done.
-      apply lookup_lt_Some in Hsome. split;[apply Z.leb_le|apply Z.ltb_lt]; solve_addr. }
+      apply lookup_lt_Some in Hsome. split;[apply Z.leb_le|apply Z.ltb_lt]; solve_addr.
+    }
     (* store_z r_t1 v1 *)
     destruct l; [inversion Hlength|].
     destruct acta as [| a0 acta]; [inversion Hact_len_a|].
     assert (a0 = act_b) as ->.
-    { feed pose proof (finz_seq_between_first act_b act_e) as HH. solve_addr.
+    { opose proof (finz_seq_between_first act_b act_e _) as HH; first solve_addr.
       rewrite -Heqacta /= in HH. by inversion HH. }
     iDestruct "Hact" as "[Ha0 Hact]".
     iPrologue "Hprog".
@@ -1857,7 +1830,7 @@ Section macros.
       revert Hcont Hcont_rest Hmid; clear. solve_addr. }
     { rewrite !dom_insert_L. rewrite Hrmap_dom.
       repeat (rewrite singleton_union_difference_L all_registers_union_l).
-      f_equal. clear; set_solver. }
+      f_equal. }
     iNext. iIntros "(HPC & Hmalloc_prog & Hpc_b & Ha_entry & Hbe & Hr_t0 & Hna & Hregs)".
     iDestruct "Hbe" as (b e Hbe) "(Hr_t1 & Hbe)".
     rewrite delete_insert_delete.
