theories/ftlr_binary/interp_weakening.v
@@ -27,14 +27,6 @@ Section fundamental.
                       -∗ □ spec_ctx
                       -∗ □ interp (WCap a1 a2 a3 a4, WCap a1 a2 a3 a4) -∗ interp_conf))%I.
 
-  (* TODO: Move somewhere ?*)
-  Lemma PermFlowsToPermFlows p p':
-    PermFlowsTo p p' <-> PermFlows p p'.
-  Proof.
-    rewrite /PermFlows; split; intros; auto.
-    destruct (Is_true_reflect (PermFlowsTo p p')); auto.
-  Qed.
-
   Instance if_persistent (PROP: bi) (b: bool) (φ1 φ2: PROP) (H1: Persistent φ1) (H2: Persistent φ2):
     Persistent (if b then φ1 else φ2).
   Proof.
