theories/rules/rules_Jnz.v
@@ -167,7 +167,6 @@ Section cap_lang_rules.
     iIntros (Hinstr Hvpc ϕ) "(>HPC & >Hpc_a) Hφ".
     iDestruct (map_of_regs_1 with "HPC") as "Hmap".
     iApply (wp_Jnz with "[$Hmap Hpc_a]"); eauto; simplify_map_eq; eauto.
-    by unfold regs_of; rewrite !dom_insert; set_solver+.
     iNext. iIntros (regs' retv) "(#Hspec & Hpc_a & Hmap)". iDestruct "Hspec" as %Hspec.
 
    destruct Hspec as [ | | ]; [ by simplify_map_eq .. | ].
