theories/rules_binary/rules_binary_Load.v
@@ -37,8 +37,8 @@ Section cap_lang_spec_rules.
     (* Derive necessary register values in r *)
      pose proof (lookup_weaken _ _ _ _ HPC Hregs).
      specialize (indom_regs_incl _ _ _ Dregs Hregs) as Hri. unfold regs_of in Hri.
-     feed destruct (Hri r2) as [r2v [Hr'2 Hr2]]. by set_solver+.
-     feed destruct (Hri r1) as [r1v [Hr'1 _]]. by set_solver+. clear Hri.
+     odestruct (Hri r2) as [r2v [Hr'2 Hr2]]. by set_solver+.
+     odestruct (Hri r1) as [r1v [Hr'1 _]]. by set_solver+. clear Hri.
      (* Derive the PC in memory *)
      iDestruct (memspec_heap_valid_inSepM _ _ _ _ pc_a with "Hown Hmem") as %Hma; eauto.
 
