theories/stdpp_extra.v
@@ -37,20 +37,6 @@ Proof.
   simpl. destruct (decide (P x)); rewrite /filter; try congruence.
 Qed.
 
-Lemma dom_map_imap_full {K A B}
-      `{Countable A, EqDecision A, Countable B, EqDecision B, Countable K, EqDecision K}
-      (f: K -> A -> option B) (m: gmap K A):
-  (∀ k a, m !! k = Some a → is_Some (f k a)) →
-  dom (map_imap f m) = dom m.
-Proof.
-  intros Hf.
-  apply set_eq. intros k.
-  rewrite !elem_of_dom map_lookup_imap.
-  destruct (m !! k) eqn:Hmk.
-  - destruct (Hf k a Hmk) as [? Hfk]. cbn. rewrite Hfk. split; eauto.
-  - cbn. split; inversion 1; congruence.
-Qed.
-
 Lemma dom_list_to_map_singleton {K V: Type} `{EqDecision K, Countable K} (x:K) (y:V):
   dom (list_to_map [(x, y)] : gmap K V) = list_to_set [x].
 Proof. rewrite dom_insert_L /= dom_empty_L. set_solver. Qed.
@@ -220,14 +206,14 @@ Lemma difference_het_lookup_Some
     {A B C} `{Countable A, EqDecision A, Countable B, EqDecision B}
     (m1: gmap A B) (m2: gmap A C) (k: A) (v: B):
   (m1 ∖∖ m2) !! k = Some v ↔ m1 !! k = Some v ∧ m2 !! k = None.
-Proof. by rewrite /map_difference_het map_filter_lookup_Some. Qed.
+Proof. by rewrite /map_difference_het map_lookup_filter_Some. Qed.
 
 Lemma difference_het_lookup_None
     {A B C} `{Countable A, EqDecision A, Countable B, EqDecision B}
     (m1: gmap A B) (m2: gmap A C) (k: A) (v: B):
   (m1 ∖∖ m2) !! k = None ↔ m1 !! k = None ∨ is_Some (m2 !! k).
 Proof.
-  rewrite /map_difference_het map_filter_lookup_None.
+  rewrite /map_difference_het map_lookup_filter_None.
   split; intros [HH1|HH2]; eauto.
   { destruct (m1 !! k) eqn:?; eauto; right.
     destruct (m2 !! k) eqn:?; eauto. exfalso. eapply HH2; eauto. }
@@ -241,7 +227,7 @@ Lemma difference_het_empty
   m ∖∖ (∅ : gmap A C) = m.
 Proof.
   rewrite /map_difference_het map_eq'. intros k v.
-  rewrite map_filter_lookup_Some. rewrite lookup_empty. set_solver.
+  rewrite map_lookup_filter_Some. rewrite lookup_empty. set_solver.
 Qed.
 
  Lemma difference_het_eq_empty
@@ -250,7 +236,7 @@ Qed.
   m ∖∖ m = (∅ : gmap A B).
 Proof.
   rewrite /map_difference_het map_eq'. intros k v.
-  rewrite map_filter_lookup_Some. rewrite lookup_empty. set_solver.
+  rewrite map_lookup_filter_Some. rewrite lookup_empty. set_solver.
 Qed.
 
 Lemma difference_het_insert_r
@@ -260,8 +246,8 @@ Lemma difference_het_insert_r
 Proof.
   intros.
   rewrite /map_difference_het map_eq'. intros k' v'.
-  rewrite map_filter_lookup_Some lookup_delete_Some.
-  rewrite map_filter_lookup_Some lookup_insert_None. set_solver.
+  rewrite map_lookup_filter_Some lookup_delete_Some.
+  rewrite map_lookup_filter_Some lookup_insert_None. set_solver.
 Qed.
 
 Lemma difference_het_insert_l
@@ -272,9 +258,9 @@ Lemma difference_het_insert_l
 Proof.
   intros.
   rewrite /map_difference_het map_eq'. intros k' v'.
-  rewrite map_filter_lookup_Some lookup_insert_Some.
+  rewrite map_lookup_filter_Some lookup_insert_Some.
   rewrite -map_filter_insert_True;auto.
-    by rewrite map_filter_lookup_Some lookup_insert_Some.
+    by rewrite map_lookup_filter_Some lookup_insert_Some.
 Qed.
 
 Lemma difference_het_delete_assoc
@@ -284,9 +270,9 @@ Lemma difference_het_delete_assoc
 Proof.
   intros.
   rewrite /map_difference_het map_eq'. intros k' v'.
-  rewrite map_filter_lookup_Some.
+  rewrite map_lookup_filter_Some.
   rewrite -map_filter_delete;auto.
-  rewrite map_filter_lookup_Some. set_solver.
+  rewrite map_lookup_filter_Some. set_solver.
 Qed.
 
 Lemma dom_difference_het
@@ -607,6 +593,33 @@ Proof.
   - cbn [create_gmap_default list_to_set]. rewrite dom_insert_L // IHl //.
 Qed.
 
+Lemma create_gmap_default_lookup_None {K V : Type} `{Countable K}
+  (l : list K) (d : V) (k : K) :
+  k ∉ l →
+  (create_gmap_default l d) !! k = None.
+Proof.
+  intros Hk.
+  induction l;auto.
+  simpl. apply not_elem_of_cons in Hk as [Hne Hk].
+  rewrite lookup_insert_ne//. apply IHl. auto.
+Qed.
+
+Lemma create_gmap_default_permutation {K V : Type} `{Countable K}
+  (l l' : list K) (d : V) :
+  l ≡ₚ l' →
+  (create_gmap_default l d) = (create_gmap_default l' d).
+Proof.
+  intros Hperm.
+  apply map_eq. intros k.
+  destruct (decide (k ∈ l)).
+  - assert (k ∈ l') as e';[rewrite -Hperm;auto|].
+    apply (create_gmap_default_lookup _ d) in e as ->.
+    apply (create_gmap_default_lookup _ d) in e' as ->. auto.
+  - assert (k ∉ l') as e';[rewrite -Hperm;auto|].
+    apply (create_gmap_default_lookup_None _ d) in n as ->.
+    apply (create_gmap_default_lookup_None _ d) in e' as ->. auto.
+Qed.
+
 Lemma fst_zip_prefix A B (l : list A) (k : list B) :
   (zip l k).*1 `prefix_of` l.
 Proof.
@@ -681,9 +694,9 @@ Proof.
 Qed.
 
 Lemma map_to_list_delete {A B} `{Countable A} `{EqDecision A} (m : gmap A B) (i : A) (x : B) :
-  ∀ l, (i,x) :: l ≡ₚmap_to_list m ->
+  ∀ l, (i,x) :: l ≡ₚ map_to_list m ->
        NoDup (i :: l.*1) →
-       (map_to_list (delete i m)) ≡ₚl.
+       (map_to_list (delete i m)) ≡ₚ l.
 Proof.
   intros l Hl Hdup.
   assert ((i,x) ∈ map_to_list m) as Hin.
@@ -731,9 +744,9 @@ Proof.
 Qed.
 
 Lemma map_to_list_delete_fst {A B} `{Countable A} (m : gmap A B) (i : A) (x : B) :
-  ∀ l, i :: l ≡ₚ(map_to_list m).*1 ->
+  ∀ l, i :: l ≡ₚ (map_to_list m).*1 ->
        NoDup (i :: l) →
-       (map_to_list (delete i m)).*1 ≡ₚl.
+       (map_to_list (delete i m)).*1 ≡ₚ l.
 Proof.
   intros l Hl Hdup.
   assert (i ∈ (map_to_list m).*1) as Hin.
@@ -908,3 +921,118 @@ Proof.
     simpl. rewrite rev_unit. rewrite rev_involutive. rewrite -Hsome /=.
     f_equiv. rewrite firstn_all. auto.
 Qed.
+
+
+
+Definition prod_op {A B : Type} :=
+  λ (o1 : option A) (o2 : option B),
+    match o1 with
+    | Some b =>
+        match o2 with
+        | Some c => Some (b,c)
+        | None => None
+        end
+    | None => None
+    end.
+
+Definition prod_merge {A B C : Type} `{Countable A} : gmap A B → gmap A C → gmap A (B * C) :=
+  λ m1 m2, merge prod_op m1 m2.
+
+(* TODO: integrate into stdpp? *)
+Lemma pair_eq_inv {A B} {y u : A} {z t : B} {x} :
+    x = (y, z) -> x = (u, t) ->
+    y = u ∧ z = t.
+Proof. intros ->. inversion 1. auto. Qed.
+
+Tactic Notation "simplify_pair_eq" :=
+  repeat
+    lazymatch goal with
+    | H1 : ?x = (?y, ?z), H2 : ?x = (?u, ?t) |- _ =>
+      assert (y = u ∧ z = t) as [? ?] by (exact (pair_eq_inv H1 H2)); clear H2
+    | H1 : (?y, ?z) = ?x, H2 : ?x = (?u, ?t) |- _ =>
+      assert (y = u ∧ z = t) as [? ?] by (exact (pair_eq_inv (eq_sym H1) H2)); clear H2
+    | H1 : ?x = (?y, ?z), H2 : (?u, ?t) = ?x |- _ =>
+      assert (y = u ∧ z = t) as [? ?] by (exact (pair_eq_inv H1 (eq_sym H2))); clear H2
+    | H1 : (?y, ?z) = ?x, H2 : (?u, ?t) = ?x |- _ =>
+      assert (y = u ∧ z = t) as [? ?] by (exact (pair_eq_inv (eq_sym H1) (eq_sym H2))); clear H2
+    | |- _ => progress simplify_eq
+    end.
+
+(*----------------------- FIXME TEMPORARY ------------------------------------*)
+(* This is a copy-paste from stdpp (fin_maps.v), plus a fix to avoid using
+   "rewrite .. by .." that is not available when using ssreflect's rewrite. *)
+(* TODO: upstream the fix into stdpp, and remove the code below whenever we
+   upgrade to a version of stdpp that includes it *)
+
+Tactic Notation "simpl_map" "by" tactic3(tac) := repeat
+  match goal with
+  | H : context[ ∅ !! _ ] |- _ => rewrite lookup_empty in H
+  | H : context[ (<[_:=_]>_) !! _ ] |- _ =>
+    rewrite lookup_insert in H || (rewrite lookup_insert_ne in H; [| by tac])
+  | H : context[ (alter _ _ _) !! _] |- _ =>
+    rewrite lookup_alter in H || (rewrite lookup_alter_ne in H; [| by tac])
+  | H : context[ (delete _ _) !! _] |- _ =>
+    rewrite lookup_delete in H || (rewrite lookup_delete_ne in H; [| by tac])
+  | H : context[ {[ _ := _ ]} !! _ ] |- _ =>
+    rewrite lookup_singleton in H || (rewrite lookup_singleton_ne in H; [| by tac])
+  | H : context[ (_ <$> _) !! _ ] |- _ => rewrite lookup_fmap in H
+  | H : context[ (omap _ _) !! _ ] |- _ => rewrite lookup_omap in H
+  | H : context[ lookup (A:=?A) ?i (?m1 ∪ ?m2) ] |- _ =>
+    let x := fresh in evar (x:A);
+    let x' := eval unfold x in x in clear x;
+    let E := fresh in
+    assert ((m1 ∪ m2) !! i = Some x') as E by (clear H; by tac);
+    rewrite E in H; clear E
+  | |- context[ ∅ !! _ ] => rewrite lookup_empty
+  | |- context[ (<[_:=_]>_) !! _ ] =>
+    rewrite lookup_insert || (rewrite lookup_insert_ne; [| by tac])
+  | |- context[ (alter _ _ _) !! _ ] =>
+    rewrite lookup_alter || (rewrite lookup_alter_ne; [| by tac])
+  | |- context[ (delete _ _) !! _ ] =>
+    rewrite lookup_delete || (rewrite lookup_delete_ne; [| by tac])
+  | |- context[ {[ _ := _ ]} !! _ ] =>
+    rewrite lookup_singleton || (rewrite lookup_singleton_ne; [| by tac])
+  | |- context[ (_ <$> _) !! _ ] => rewrite lookup_fmap
+  | |- context[ (omap _ _) !! _ ] => rewrite lookup_omap
+  | |- context [ lookup (A:=?A) ?i ?m ] =>
+    let x := fresh in evar (x:A);
+    let x' := eval unfold x in x in clear x;
+    let E := fresh in
+    assert (m !! i = Some x') as E by tac;
+    rewrite E; clear E
+  end.
+
+Tactic Notation "simpl_map" := simpl_map by eauto with simpl_map map_disjoint.
+
+Tactic Notation "simplify_map_eq" "by" tactic3(tac) :=
+  decompose_map_disjoint;
+  repeat match goal with
+  | _ => progress simpl_map by tac
+  | _ => progress simplify_eq/=
+  | _ => progress simpl_option by tac
+  | H : {[ _ := _ ]} !! _ = None |- _ => rewrite lookup_singleton_None in H
+  | H : {[ _ := _ ]} !! _ = Some _ |- _ =>
+    rewrite lookup_singleton_Some in H; destruct H
+  | H1 : ?m1 !! ?i = Some ?x, H2 : ?m2 !! ?i = Some ?y |- _ =>
+    let H3 := fresh in
+    opose proof (lookup_weaken_inv m1 m2 i x y) as H3; [done|by tac|done|];
+    clear H2; symmetry in H3
+  | H1 : ?m1 !! ?i = Some ?x, H2 : ?m2 !! ?i = None |- _ =>
+    let H3 := fresh in
+    apply (lookup_weaken _ m2) in H1; [congruence|by tac]
+  | H : ?m ∪ _ = ?m ∪ _ |- _ =>
+    apply map_union_cancel_l in H; [|by tac|by tac]
+  | H : _ ∪ ?m = _ ∪ ?m |- _ =>
+    apply map_union_cancel_r in H; [|by tac|by tac]
+  | H : {[?i := ?x]} = ∅ |- _ => by destruct (map_non_empty_singleton i x)
+  | H : ∅ = {[?i := ?x]} |- _ => by destruct (map_non_empty_singleton i x)
+  | H : ?m !! ?i = Some _, H2 : ?m !! ?j = None |- _ =>
+     unless (i ≠ j) by done;
+     assert (i ≠ j) by (by intros ?; simplify_eq)
+  end.
+Tactic Notation "simplify_map_eq" "/=" "by" tactic3(tac) :=
+  repeat (progress csimpl in * || simplify_map_eq by tac).
+Tactic Notation "simplify_map_eq" :=
+  simplify_map_eq by eauto with simpl_map map_disjoint.
+Tactic Notation "simplify_map_eq" "/=" :=
+  simplify_map_eq/= by eauto with simpl_map map_disjoint.
